saving the new thoughts

prototype/unstacked_borrows_pseudo.dfy
@@ -5,65 +5,73 @@ class State {
    var counter: nat; // used to generate new id
    var mem: array<int>;
    var tagmem: array<Tag>;
+   var predecessor: array<int>;
    
    // the tag from which a raw ponter borrows from
    var rawfrom: array<int>;  
 
    constructor(mem: array<int>)
-   ensures fresh(tagmem) && fresh(rawfrom);
+   ensures fresh(tagmem) && fresh(rawfrom) && fresh(predecessor);
    ensures this.mem == mem && counter == 0;
    ensures forall i:: 0 <= i && i < tagmem.Length ==> tagmem[i] == Owner;
    ensures forall i:: 0 <= i && i < rawfrom.Length ==> rawfrom[i] == -1;
+   ensures forall i:: 0 <= i && i < predecessor.Length ==> predecessor[i] == -1;
+   ensures rawfrom != predecessor && mem!= predecessor;
    ensures valid();
    {
      this.mem := mem;
      tagmem := new Tag[mem.Length](_ => Owner);
      rawfrom := new int[mem.Length](_ => -1);
+     predecessor := new int[mem.Length](_ =>-1);
      counter := 0;
      
    }
 
    predicate valid()
-   reads this, mem, tagmem, rawfrom;
+   reads this, mem, tagmem, rawfrom, predecessor;
    {
-    mem.Length == tagmem.Length && mem.Length == rawfrom.Length 
-    && forall i:: 0 <= i && i < tagmem.Length && tagmem[i].Unique? ==> tagmem[i].t <= counter
+    rawfrom != predecessor && mem != predecessor && rawfrom != mem &&
+    mem.Length == tagmem.Length && mem.Length == rawfrom.Length &&
+    mem.Length == predecessor.Length && predecessor != rawfrom &&
+    (forall i:: 0 <= i && i < tagmem.Length && tagmem[i].Unique? ==> 
+          predecessor[i] < tagmem[i].t && tagmem[i].t <= counter)  &&
+    (forall i:: 0 <= i && i < tagmem.Length && tagmem[i].SharedRO? ==> 
+          predecessor[i] < tagmem[i].t && tagmem[i].t <= counter)   
    } 
 
    predicate valid_addr(addr: int)
    requires valid();
-   reads this, mem,tagmem, rawfrom;
+   reads this, mem,tagmem, rawfrom, predecessor;
    {
       0 <= addr && addr < mem.Length
    }
 
-predicate invalidTag(addr: nat, tag: Tag, predecessor: Tag)
+predicate invalidTag(addr: nat, tag: Tag, predece: int)
  requires valid() && valid_addr(addr);
- reads this, tagmem, rawfrom, mem;
+ requires tag.Unique? ==>  predece < tag.t;
+ reads this, tagmem, rawfrom, mem, predecessor;
  {
-    match (tagmem[addr], tag, predecessor)
-    case (Unique(n1, c1), Unique(n2, c2),  Unique(n3, c3)) => 
+    match (tagmem[addr], tag, predece)
+    case (Unique(n1, c1), Unique(n2, c2),  n3) => 
      if (rawfrom[addr] != -1) then n2 != n1
       else n1 < n2 || (n1 > n2 && n3 <= n1)
     case (SharedRO(n1, c1), Unique(n2, c2), _) => 
      if (rawfrom[addr] != -1) then true 
      else false  // unknown
     case (Unique(n1, c1), SharedRO(n2, c2), _) => n2 < n1
-    case (SharedRO(n1, c1), SharedRO(n2, c2), _) => false  // unknown
+    case (SharedRO(n1, c1), SharedRO(n2, c2), n3) =>   
+          n3 < n1 // fixme
     case (Owner, _, _) => false
     case (_, _, _) => true
 }  
 
-predicate validTag(addr: nat, tag: Tag, predecessor: Tag)
+predicate validTag(addr: nat, tag: Tag, predece: int)
 requires valid() && valid_addr(addr);
-reads this, tagmem, rawfrom, mem;
+requires tag.Unique? ==>  predece < tag.t;
+reads this, tagmem, rawfrom, mem, predecessor;
 {
-   (tag.Unique?  ==> tag.t <= counter) && 
-   (
-     tagmem[addr] == Owner 
-     ||  
-     (tagmem[addr] != Owner ==> !invalidTag(addr, tag, predecessor))
-   )
+   (tag.Unique?  ==> tag.t <= counter && !invalidTag(addr, tag, predece)) && 
+   (tag.SharedRO? ==> tag.t <= counter && !invalidTag(addr, tag, predece))
 }
     
    
@@ -71,7 +79,7 @@ reads this, tagmem, rawfrom, mem;
    requires valid();
    modifies this;
    ensures counter == old(counter) + 1 && ret == counter;
-   ensures mem == old(mem) && tagmem == old(tagmem) && rawfrom == old(rawfrom);
+   ensures mem == old(mem) && tagmem == old(tagmem) && rawfrom == old(rawfrom) && predecessor == old(predecessor);
    ensures forall i:: 0 <= i && i < tagmem.Length && tagmem[i].Unique? ==> tagmem[i].t < ret; 
    ensures valid();
    {
@@ -82,33 +90,24 @@ reads this, tagmem, rawfrom, mem;
    predicate isWritable(p: Pointer)
    requires valid();
    requires p.valid(this);
-   reads this, mem, rawfrom, tagmem, p;
+   requires p.tag.Unique?;
+   reads this, mem, rawfrom, tagmem, predecessor, p;
    { 
-      match p.tag
-      case Unique(t, c)  => true
-      case _ => false
-   }
-   
-   predicate valid_predecessor(tag: Tag, predec: Tag)
-   reads this;
-   {
-     match (tag, predec)
-       case (Unique(n1, c1), Unique(n2, c2)) =>  n2 < n1
-       case (SharedRO(n1, c1), Unique(n2, c2)) => n2 < n1
-       case (_, Owner) => true
-       case _ => false 
+      validTag(p.addr, p.tag, p.predecessor)
    }
    
   method write(p: Pointer, v: int)
      requires valid();
-     // requires p.valid(this) && isWritable(p);
-     requires valid_addr(p.addr) && p.tag.Unique?;
+     requires p.valid(this) && p.tag.Unique? && isWritable(p);
+    //  requires valid_addr(p.addr) && p.tag.Unique?;
      requires p.tag.Unique? ==> p.tag.t <= counter;
-     modifies mem, tagmem, rawfrom;
+     modifies this, mem, tagmem, rawfrom, predecessor;
+     ensures mem == old(mem) && tagmem == old(tagmem)  && rawfrom == old(rawfrom) && predecessor == old(predecessor) && counter == old(counter);
      ensures forall i :: 0 <= i && i < tagmem.Length && i != p.addr ==> tagmem[i] == old(tagmem[i]);
      ensures forall i :: 0 <= i && i < mem.Length && i != p.addr ==> mem[i] == old(mem[i]);
      ensures forall i :: 0 <= i && i < rawfrom.Length && i != p.addr ==> rawfrom[i] == old(rawfrom[i]);
-     ensures p.tag.Unique? ==> tagmem[p.addr] == p.tag;
+     ensures forall i :: 0 <= i && i < predecessor.Length && i != p.addr ==> predecessor[i] == old(predecessor[i]);
+     ensures p.tag.Unique? ==> tagmem[p.addr] == p.tag && predecessor[p.addr] == p.predecessor;
      ensures mem[p.addr] == v;
      ensures valid();
    {
@@ -116,31 +115,46 @@ reads this, tagmem, rawfrom, mem;
      case Unique(t, c) =>
        mem[p.addr] := v;
        tagmem[p.addr] := p.tag;
+       predecessor[p.addr] := p.predecessor;
      
    }
-   
-   
+   /*
+   predicate isReadble(p: Pointer)
+   requires valid();
+   requires p.valid(this);
+   requires p.tag.Unique? || p.tag.SharedRO?
+   reads this, mem, rawfrom, tagmem, predecessor, p;
+   { 
+      validTag(p.addr, p.tag, p.predecessor)
+
+   }
+
    method read(p: Pointer) returns (r: int)
    requires valid();
-   // requires p.valid(this);
-   requires valid_addr(p.addr);
-   modifies tagmem;
+   requires p.valid(this) && (p.tag.Unique? || p.tag.SharedRO?) && isReadble(p);
+   // requires valid_addr(p.addr);
+   requires p.tag.Unique? ==> p.tag.t <= counter;
+   modifies tagmem, predecessor;
    ensures forall i :: 0 <= i && i < tagmem.Length && i != p.addr ==> tagmem[i] == old(tagmem[i]);
-   ensures forall i :: 0 <= i && i < mem.Length && i != p.addr ==> mem[i] == old(mem[i]);
+   // ensures forall i :: 0 <= i && i < mem.Length && i != p.addr ==> mem[i] == old(mem[i]);
    ensures forall i :: 0 <= i && i < rawfrom.Length && i != p.addr ==> rawfrom[i] == old(rawfrom[i]);
-   ensures p.tag.Unique? ==> tagmem[p.addr] == p.tag;
+   ensures forall i :: 0 <= i && i < predecessor.Length && i != p.addr ==> predecessor[i] == old(predecessor[i]);
+   ensures p.tag.Unique? ==> tagmem[p.addr] == p.tag && predecessor[p.addr] == p.predecessor;
    ensures valid();
    {
      r := mem[p.addr];
      match p.tag
      case Unique(t, c) =>
         tagmem[p.addr] := p.tag;
+        predecessor[p.addr] := p.predecessor;
      case SharedRO(t, c) =>
       // nothing to do
      
      case _ => // ?
    }
-   
+
+   */
+  
 } 
   
 
@@ -149,24 +163,27 @@ reads this, tagmem, rawfrom, mem;
 class Pointer{
   var addr: nat;
   var tag: Tag;
-  var predecessor: Tag; // the upperbound of the predecessor
+  // can we treated as the upperbound of the predecessor
+  var predecessor: int; 
   
  predicate valid(s: State)
  requires s.valid();
- reads s, s.tagmem, s.rawfrom, s.mem, this;
+ reads s, s.tagmem, s.rawfrom, s.mem, s.predecessor, this;
  {
-    s.valid_addr(addr) && s.valid_predecessor(this.tag, this.predecessor) &&
-    s.validTag(addr, tag, predecessor) 
+    s.valid_addr(addr) && 
+    (tag.Unique? ==> predecessor < tag.t && s.validTag(addr, tag, predecessor)) &&
+    (tag.SharedRO? ==> predecessor < tag.t && s.validTag(addr, tag, predecessor))
  }
 
- 
- 
- constructor(addr: nat, tag: Tag, predecessor: Tag, s: State) 
+  
+ constructor(addr: nat, tag: Tag, predecessor: int, s: State) 
   requires s.valid() && s.valid_addr(addr);
-  requires s.validTag(addr, tag, predecessor) && s.valid_predecessor(tag, predecessor);
-  // requires tag.Unique? ==> tag.t == s.counter;
-  ensures this.addr == addr && this.tag == tag && /* this.predecessor == predecessor */ s.valid_predecessor(tag, this.predecessor); // under specified
-  // ensures this.addr == addr && this.tag == tag && this.predecessor == predecessor;
+  requires tag.Unique? || tag.SharedRO?;
+  requires tag.Unique?  ==> predecessor < tag.t && tag.t == s.counter;
+  requires tag.SharedRO? ==> predecessor <  tag.t && tag.t == s.counter;
+  requires s.validTag(addr, tag, predecessor);
+  // ensures this.addr == addr && this.tag == tag; // under specified
+   ensures this.addr == addr && this.tag == tag && this.predecessor == predecessor;
   ensures valid(s);
   {
     this.addr := addr;
@@ -175,15 +192,18 @@ class Pointer{
   }
 }
 
+/*-----------------Unique------------------------------------------------*/
+
 method createMutableRef(p: Pointer, s: State) returns(ret: Pointer)
 requires s.valid() &&  s.valid_addr(p.addr) /* p.valid(s) */ && p.tag.Unique?;
 requires p.tag.Unique? ==> p.tag.t <= s.counter;
-modifies s, s.tagmem, s.rawfrom;
-ensures s.tagmem == old(s.tagmem) && s.mem == old(s.mem) && s.rawfrom == old(s.rawfrom);
+modifies s, s.tagmem, s.rawfrom, s.predecessor;
+ensures s.tagmem == old(s.tagmem)  && s.rawfrom == old(s.rawfrom) && s.predecessor == old(s.predecessor);
 ensures s.counter == old(s.counter) + 1;
 ensures forall i :: 0 <= i && i < s.tagmem.Length && i != p.addr ==> s.tagmem[i] == old(s.tagmem[i]);
 ensures forall i :: 0 <= i && i < s.rawfrom.Length && i != p.addr ==> s.rawfrom[i] == old(s.rawfrom[i]);
-ensures s.tagmem[p.addr] == ret.tag && s.rawfrom[p.addr] == -1;
+ensures forall i :: 0 <= i && i < s.predecessor.Length && i != p.addr ==> s.predecessor[i] == old(s.predecessor[i]);
+ensures s.tagmem[p.addr] == ret.tag && s.rawfrom[p.addr] == -1 && s.predecessor[p.addr] == p.tag.t;
 ensures ret.addr == p.addr && ret.tag == Unique(s.counter, p.tag.c);
 ensures fresh(ret);
 ensures s.valid() && ret.valid(s);
@@ -195,8 +215,8 @@ ensures s.valid() && ret.valid(s);
        var newtag := Unique(newID, c?);
        s.tagmem[p.addr] := newtag;
        s.rawfrom[p.addr] := -1;
-       assert newID > t;
-       ret := new Pointer(p.addr, newtag, p.tag, s);
+       s.predecessor[p.addr] := t;
+       ret := new Pointer(p.addr, newtag, t, s);
    // case _ =>
    //    ret := new Pointer(p.addr, Disabled, s);
        // todo
@@ -205,59 +225,67 @@ ensures s.valid() && ret.valid(s);
 
 // This client follows stack principle
 // C1
-method mutableTest1(mem:array<int>)
-  modifies mem;
+// s
+
+/*---------------SharedRO---------------------------------*/
+/*
+Rule (NEW-SHARE-REF-1)
+*/
+/*
+method createSharedRO(p: Pointer, s: State) returns(ret: Pointer)
+requires s.valid() && s.valid_addr(p.addr);
+//requires p.valid(s);
+requires  (p.tag.Unique? || p.tag.SharedRO?);
+requires p.tag.Unique? ==> p.tag.t <= s.counter;
+requires p.tag.SharedRO? ==> p.tag.t <= s.counter && p.predecessor.Unique? && p.predecessor.t < s.counter;
+modifies s, s.tagmem, s.rawfrom;
+ensures s.tagmem == old(s.tagmem) && s.mem == old(s.mem) && s.rawfrom == old(s.rawfrom);
+ensures s.counter == old(s.counter) + 1;
+ensures forall i :: 0 <= i && i < s.tagmem.Length && i != p.addr ==> s.tagmem[i] == old(s.tagmem[i]);
+ensures forall i :: 0 <= i && i < s.rawfrom.Length  ==> s.rawfrom[i] == old(s.rawfrom[i]);
+ensures ret.addr == p.addr && ret.tag == SharedRO(s.counter, p.tag.c);
+ensures p.tag.Unique? ==> ret.predecessor == p.tag;
+ensures p.tag.SharedRO? ==> ret.predecessor == p.predecessor;
+ensures fresh(ret);
+ensures s.valid() && ret.valid(s);
 {
-  var s := new State(mem);
-      
-  // let mut local1 = 5;
-  var local1: nat;
-  var tag1 := s.generateID();
-  if(0 < local1 < mem.Length){
-    mem[local1] := 5;
-    
-    
-    var ref1: Pointer := new Pointer(local1, Unique(tag1, 1), Owner, s);
-     assert ref1.tag.Unique?;
-    
-    // let x = & mut local;
-    var ref2: Pointer := createMutableRef(ref1, s);
-    
-    // let y = & mut local;
-    var ref3: Pointer := createMutableRef(ref1, s);
-    
-    assert s.tagmem[local1].Unique? && ref1.tag.Unique?;
-    assert s.tagmem[local1].Unique? && ref1.tag.Unique? ==> ref1.tag.t < s.tagmem[local1].t;
-    assert(!ref1.valid(s));
-  
-    
-  }
+  var newID := s.generateID();
+  var newtag := SharedRO(newID, p.tag.c);
+  match p.tag
+  case Unique(t, c?) =>
+    s.tagmem[p.addr] := newtag;
+    ret := new Pointer(p.addr, newtag, p.tag, s);
+  case SharedRO(t, c?) =>
+    // not update the top
+    // inherit top's predecessor
+     assert newtag.SharedRO? && (p.predecessor.Unique? || p.predecessor.Owner?);
+     assert newtag.SharedRO? && p.predecessor.Unique? ==> newtag.t > p.predecessor.t;
+    ret := new Pointer(p.addr, newtag, p.predecessor, s);
 }
 
-// C2
-method mutableTest2(mem:array<int>)
-  modifies mem;
+method SharedROTest(mem:array<int>)
+modifies mem;
 {
   var s := new State(mem);
-      
+        
   // let mut local1 = 5;
   var local1: nat;
   var tag1 := s.generateID();
   if(0 < local1 < mem.Length){
-    mem[local1] := 5;
-    // let x = & mut local1
-    var ref1: Pointer := new Pointer(local1, Unique(tag1, 1), Owner, s);
-    
-    // let x = & mut local;
-    var ref2: Pointer := createMutableRef(ref1, s);
-    
-    // let y = & mut *x
-    var ref3: Pointer := createMutableRef(ref2, s);
-       
-    // write(x)
-    s.write(ref2, 42);
-    
-    assert !ref3.valid(s);
+      mem[local1] := 5;
+      var ref1: Pointer := new Pointer(local1, Unique(tag1, 1), Owner, s);
+     
+      // let x = & mut local;
+      var ref2: Pointer := createMutableRef(ref1, s);
+      
+      // let y = & x;
+      var ref3: Pointer := createSharedRO(ref2, s);
+      assert(ref3.valid(s));
+      var ref4: Pointer := createSharedRO(ref2, s);
+      assert(ref4.valid(s));
+      var ref5: Pointer := createMutableRef(ref2, s);
+      assert(!ref4.valid(s));
+
   }
-  
 }
+*/
